low-equivalence && expression equivalence

while-program-infoflow/VSITypeSoundness.dfy
@@ -57,4 +57,66 @@ module VSISoundness {
 
     /**  We prove the information flow security is enforced by the VSI type checking
      */
+    // Low equivalent states
+    predicate LowEquiv(ctx: Context, s1: MState, s2: MState)
+    requires ctx.Keys == s1.Keys == s2.Keys
+    {
+        forall x :: x in ctx.Keys && ctx[x] == Low ==> s1[x] == s2[x]
+    }
+    // First, we show that every expression (not Cmd) has a valid type
+    lemma ValidExprType(ctx: Context, e: Expr)
+    requires VariablesInExpr(e) <= ctx.Keys
+    requires forall x :: x in ctx.Keys ==> ctx[x] != InvalidBase
+    ensures HasExprType(ctx, e) != Invalid
+    ensures GetBaseType(HasExprType(ctx, e)) != InvalidBase
+    {}
+    // If e is typed Low, then e only contains variables of type Low *** 
+    lemma {:induction false} SimpleSecurity(ctx: Context, e: Expr, x: Variable)
+    requires VariablesInExpr(e) <= ctx.Keys
+    requires HasExprType(ctx, e) == ExprType(Low)
+    requires forall x :: x in ctx.Keys ==> ctx[x] != InvalidBase
+    requires x in VariablesInExpr(e) 
+    ensures ctx[x] == Low
+    {
+        match e {
+            case Num(_) => assert (! (x in VariablesInExpr(e))); assert false;
+            case Var(y) => assert x == y;
+            case Plus(e1, e2) => 
+                assert Join(GetBaseType(HasExprType(ctx, e1)), GetBaseType(HasExprType(ctx, e2))) == Low;
+                ValidExprType(ctx, e1);
+                SubTypeJoin(GetBaseType(HasExprType(ctx, e1)), Join(GetBaseType(HasExprType(ctx, e1)), GetBaseType(HasExprType(ctx, e2))));
+                assert GetBaseType(HasExprType(ctx, e1)) == Low;
+                if (x in VariablesInExpr(e1)){
+                    SimpleSecurity(ctx, e1, x);
+                } else {
+                    assert x in VariablesInExpr(e2);
+                    SimpleSecurity(ctx, e2, x);
+                }
+        }
+    }
+
+    // Low equivalent expressions
+    lemma {:induction false} LowEquivExpr(ctx: Context, s1: MState, s2: MState, e: Expr)
+    requires ctx.Keys == s1.Keys == s2.Keys
+    requires typeOK(s1) && typeOK(s2)
+    requires VariablesInExpr(e) <= ctx.Keys
+    requires forall x :: x in ctx.Keys ==> ctx[x] != InvalidBase
+    requires LowEquiv(ctx, s1, s2)
+    requires HasExprType(ctx, e) == ExprType(Low)
+    ensures Evaluate(s1, e) == Evaluate(s2, e)
+    {
+        match e {
+            case Num(_) => assert Evaluate(s1, e) == Evaluate(s2, e);
+            case Var(x) => 
+                assert ctx[x] == Low;
+            case Plus(e1, e2) => 
+                assert Join(GetBaseType(HasExprType(ctx, e1)), GetBaseType(HasExprType(ctx, e2))) == Low;
+                ValidExprType(ctx, e1);
+                SubTypeJoin(GetBaseType(HasExprType(ctx, e1)), Join(GetBaseType(HasExprType(ctx, e1)), GetBaseType(HasExprType(ctx, e2))));
+                assert HasExprType(ctx, e1) == ExprType(Low);
+                LowEquivExpr(ctx, s1, s2, e1);
+                LowEquivExpr(ctx, s1, s2, e2);
+        }
+    }
+
 }
